Replaced lenses with scenes in unrestriction and parallel substitution, as these are more flexible.

Unrestriction.thy
@@ -1,32 +1,42 @@
+section \<open> Unrestriction \<close>
+
 theory Unrestriction
   imports Expressions
 begin
 
-definition unrest :: "('a \<Longrightarrow> 's) \<Rightarrow> ('b, 's) expr \<Rightarrow> bool" where
-[expr_defs]: "unrest x e = (\<forall> s k. e (put\<^bsub>x\<^esub> s k) = e s)"
+text \<open> Unrestriction means that an expression does not depend on the value of the state space
+  described by the given scene (i.e. set of variables) for its valuation. It is a semantic
+  characterisation of fresh variables. \<close>
+
+definition unrest :: "'s scene \<Rightarrow> ('b, 's) expr \<Rightarrow> bool" where
+[expr_defs]: "unrest a e = (\<forall> s s'. e (s \<oplus>\<^sub>S s' on a) = e s)"
 
 syntax
   "_unrest" :: "salpha \<Rightarrow> logic \<Rightarrow> logic \<Rightarrow> logic" (infix "\<sharp>" 20)
 
 translations
   "_unrest x p" == "CONST unrest x (p)\<^sub>e"                                           
-  "_unrest (_salphaset (_salphamk (x +\<^sub>L y))) P"  <= "_unrest (x +\<^sub>L y) P"
 
 named_theorems unrest
 
-lemma unrest_var_comp [unrest]:
+lemma unrest_var_union [unrest]:
   "\<lbrakk> x \<sharp> P; y \<sharp> P \<rbrakk> \<Longrightarrow> x;y \<sharp> P"
   by (simp add: expr_defs lens_defs)
+     (metis scene_override_union scene_override_unit scene_union_incompat)
 
-lemma unrest_lens_comp [unrest]: "x \<sharp> e \<Longrightarrow> x:y \<sharp> e"
-  by (simp add: expr_defs lens_defs)
+lemma unrest_subscene: "\<lbrakk> idem_scene a; a \<sharp> e; b \<subseteq>\<^sub>S a \<rbrakk> \<Longrightarrow> b \<sharp> e"
+  by (metis (mono_tags, hide_lams) subscene_eliminate unrest_def)
+
+lemma unrest_lens_comp [unrest]: "\<lbrakk> vwb_lens x; vwb_lens y; &x \<sharp> e \<rbrakk> \<Longrightarrow> &x:y \<sharp> e"
+  by (simp add: expr_defs)
+     (metis comp_vwb_lens lens_comp_lb ns_alpha_def sublens_iff_subscene subscene_eliminate var_alpha_def vwb_impl_idem_scene)
 
 lemma unrest_lit [unrest]: "x \<sharp> \<guillemotleft>v\<guillemotright>"
   by (simp add: expr_defs)
 
 lemma unrest_var [unrest]:
-  "x \<bowtie> y \<Longrightarrow> x \<sharp> &y"
-  by (simp add: expr_defs lens_indep.lens_put_irr2)
+  "\<lbrakk> mwb_lens x; x \<bowtie> y \<rbrakk> \<Longrightarrow> &x \<sharp> &y"
+  by (simp add: expr_defs lens_indep.lens_put_irr2 lens_indep_sym lens_override_def lens_scene_override var_alpha_def)
 
 lemma unrest_uop [unrest]:
   "\<lbrakk> x \<sharp> e \<rbrakk> \<Longrightarrow> x \<sharp> \<guillemotleft>f\<guillemotright> e"
